

# Proof Sketch: Irrationality of $e$

## 1 The sequence $a_n = 1/n!$

**Lemma 1** (Key bound on the factorial function). *For all  $n > 0$  and  $k \in \mathbb{N}$ ,*

$$(n+k)! \geq 2^k \cdot n!.$$

*Proof.* The proof proceeds by induction on  $k$ . For the base case  $k = 0$ , we have  $(n+0)! = 2^0 \cdot n!$ . For the inductive step, assume  $(n+k)! \geq 2^k \cdot n!$ . Then

$$\begin{aligned} (n+k+1)! &= (n+k+1) \cdot (n+k)! \\ &\geq (n+k+1) \cdot 2^k \cdot n! \\ &\geq 2 \cdot 2^k \cdot n! = 2^{k+1} \cdot n!, \end{aligned}$$

where the last inequality uses that  $n+k+1 \geq 2$  when  $n > 0$ . □

Remark: the condition that  $n > 0$  cannot be dropped.

**Definition 1.** *Set  $a_n = 1/n!$ . This defines a function  $a: \mathbb{N} \rightarrow \mathbb{R}, n \mapsto a_n$ .*

**Lemma 2** (Key bound on  $a_n$ ). *For all  $n \geq 1$  and  $k \in \mathbb{N}$ , we have*

$$a_{n+k} \leq \left(\frac{1}{2}\right)^k \cdot a_n.$$

*Proof.* Follows from Lemma 1, using the fact that both sides in the inequality in Lemma 1 are positive. □

## 2 The partial sums $s_n = a_0 + \cdots + a_{n-1}$

Define the partial sums

$$s_n = \sum_{i=0}^{n-1} a_i = \frac{1}{0!} + \frac{1}{1!} + \cdots + \frac{1}{(n-1)!} \in \mathbb{R}$$

for  $n \in \mathbb{N}$ . Note that there are  $n$  terms in the sum. We follow the usual convention that  $s_0 = 0$  (empty sum).

The key inequality for the partial sums is:

**Definition 2.** *Consider the partial sum of the geometric series*

$$g_k = 1 + \frac{1}{2} + \cdots + \left(\frac{1}{2}\right)^{k-1},$$

where again  $g_0 = 0$  (empty sum).

**Lemma 3.**  $g_k < 2$ .

*Proof.* Indeed, we have  $g_k = 2 - (1/2)^{k-1}$ . □

**Lemma 4.** For all  $m$  and all  $n \geq 1$  and  $k \in \mathbb{N}$ , we have

$$s_{n+k} \leq s_n + a_n \cdot g_k.$$

*Proof.* The proof proceeds by induction on  $k$ . For  $k = 0$ , we have  $s_{n+0} = s_n + a_n \cdot g_0$ .

For the inductive step, assume  $s_{n+k} \leq s_n + a_n \cdot g_k$ . Then

$$\begin{aligned} s_{n+k+1} &= s_{n+k} + a_{n+k} \\ &\leq s_n + a_n \cdot g_k + a_{n+k} \\ &\leq s_n + a_n \cdot g_k + \left(\frac{1}{2}\right)^k \cdot a_n \\ &= s_n + a_n \cdot \left(g_k + \left(\frac{1}{2}\right)^k\right) \\ &= s_n + a_n \cdot g_{k+1}, \end{aligned}$$

where we used the bound  $a_{n+k} \leq (1/2)^k \cdot a_n$  from Lemma 2. □

**Lemma 5.** For all  $n \geq 1$  and  $k \in \mathbb{N}$ ,

$$s_{n+k} < s_n + 2 \cdot a_n.$$

*Proof.* Follows from Lemma 4 and Lemma 3. □

It will be convenient to establish the following variant:

**Lemma 6.** For all  $n \geq 1$  and all  $m \geq 0$  we have

$$s_m < s_n + 2 \cdot a_n$$

*Proof.* Follows by case distinction: if  $m > n$  then this is Lemma 5, and if  $m \leq n$  then this follows from  $s_m \leq s_n$  and  $a_n > 0$ . □

### 3 $e$ as limit of $s_n$

The number  $e$  is defined as the limit of the sequence  $(s_n)$ :

$$e = \lim_{n \rightarrow \infty} s_n = \sum_{n=0}^{\infty} \frac{1}{n!}.$$

Since  $(s_n)$  is a strictly increasing sequence (as  $a_n > 0$  for all  $n$ ) and bounded above (by Lemma 6), the limit exists.

**Lemma 7** (Characterisation of  $e$ ). *The number  $e$  satisfies:*

1. For all  $n$ , we have  $s_n < e$ ;
2. If  $c \in \mathbb{R}$  and  $s_n \leq c$  for all  $n$ , then  $e \leq c$ .

Moreover,  $e$  is the only real number that satisfies these two properties. □

Combining the second point with Lemma 6 we obtain:

**Theorem 1** (Key bound on  $e$ ). For all  $n > 0$  we have  $e \leq s_n + 2 \cdot a_n$

## 4 Proof that $n! \cdot s_{n+1}$ is an integer, but $n! \cdot e$ cannot be

Define the tail of the series:

$$t_n = e - s_n = \sum_{i=n}^{\infty} \frac{1}{i!}.$$

Note that  $t_n > 0$  for all  $n$  (since  $s_n < e$ ), and from the bound above, we have  $t_n \leq 2 \cdot a_n$  for  $n \geq 1$ .

The key ingredients are:

**Lemma 8** (Integrality of  $n! \cdot s_{n+1}$ ). *For all  $n \in \mathbb{N}$ , the number  $n! \cdot s_{n+1}$  is an integer.*

*Proof sketch.* We have

$$n! \cdot s_{n+1} = n! \cdot \sum_{i=0}^n \frac{1}{i!} = \sum_{i=0}^n \frac{n!}{i!}.$$

For  $i \leq n$ , we have  $n!/i! = n \cdot (n-1) \cdots (i+1) \in \mathbb{N}$ , so the sum is an integer.  $\square$

**Lemma 9** (Bound on  $n! \cdot t_{n+1}$ ). *For all  $n \geq 2$ ,*

$$0 < n! \cdot t_{n+1} < 1.$$

*Proof sketch.* The positivity follows from  $t_{n+1} > 0$ . For the upper bound, we use:

$$\begin{aligned} n! \cdot t_{n+1} &\leq n! \cdot 2 \cdot a_{n+1} \\ &= n! \cdot 2 \cdot \frac{1}{(n+1)!} \\ &= \frac{2}{n+1} \\ &\leq \frac{2}{3} < 1, \end{aligned}$$

where the last inequality uses  $n \geq 2$ .  $\square$

**Theorem 2** (Non-integrality of  $n! \cdot e$ ). *For all  $n \geq 2$  and any integer  $N$ , we have  $n! \cdot e \neq N$ .*

*Proof sketch.* Suppose for contradiction that  $n! \cdot e = N$  for some integer  $N$ . Since  $n! \cdot s_{n+1}$  is an integer (say  $M$ ), we have

$$n! \cdot t_{n+1} = n! \cdot (e - s_{n+1}) = N - M \in \mathbb{Z}.$$

But  $0 < n! \cdot t_{n+1} < 1$ , and there are no integers strictly between 0 and 1, which is a contradiction.  $\square$

## 5 Proof that $e$ is not rational

**Theorem 3** (Irrationality of  $e$ ). *The number  $e$  is irrational.*

*Proof sketch.* Suppose for contradiction that  $e = p/q$  for some natural numbers  $p, q$  with  $q > 0$ .

Then for  $n = q + 1 \geq 2$ , we have:

$$(q+1)! \cdot e = (q+1)! \cdot \frac{p}{q} = (q+1) \cdot q! \cdot \frac{p}{q} = (q+1) \cdot (q-1)! \cdot p \in \mathbb{N}.$$

But by the previous theorem,  $(q+1)! \cdot e$  cannot be an integer, which is a contradiction.  $\square$